Wp definition for expr

theories/program_logic/delayfree.v
@@ -1,6 +1,10 @@
 
 From stdpp Require Import list base gmap fin_sets fin_map_dom.
 From shiris.program_logic Require Import state.
+From iris.algebra Require Import auth gmap excl.
+From iris.proofmode Require Import base tactics classes.
+From iris.base_logic.lib Require Export fancy_updates.
+From shiris.program_logic Require Import delayfree.
 Require Import Unicode.Utf8.
 
 (*
@@ -10,59 +14,150 @@ This is the type algebra normalized form of:
 Do I need partiality on the get and put signatures? or can that be handled
 completely at the semantic level?
 *)
-CoInductive delayST (ST A: Type): Type :=
-| Answer: A -> delayST ST A
-| Get : (ST -> delayST ST A) -> delayST ST A
-| Put : ST -> (unit -> delayST ST A) -> delayST ST A
-| Think: delayST ST A -> delayST ST A.
+
+CoInductive itree (E: Type -> Type) (R: Type): Type :=
+| Answer (r: R) (* computation terminating with value r *)
+| Think (t: itree E R) (* "silent" tau transition with child t *)
+| Fork: itree E () ->  itree E R -> itree E R
+| Vis: ∀{A: Type}, E A ->  (A -> itree E R) -> itree E R.
 
 Arguments Answer {_ _}.
-Arguments Get {_ _}.
-Arguments Put {_ _}.
 Arguments Think {_ _}.
+Arguments Fork {_ _}.
+Arguments Vis {_ _ _}.
 
-(* Using the cofix to extract all parameters that are constant throughout the recursion
-   Is crucial in having the guardness check work for loop and iter.
-*)
-Definition delayST_bind {ST A B} 
-    (f: A -> delayST ST B):
-    ∀ (ma: delayST ST A), delayST ST B :=
-      cofix go (ma : delayST ST A) : 
-      delayST ST B :=
-        match ma with
-        | Answer x => f x
-        | Get k => Get (λ s, go (k s))
-        | Put s k => Put s (λ s, go (k tt))
-        | Think ma' => Think (go ma')
-        end.
 
-Instance mret_delayST ST: MRet (delayST ST) :=
+Definition loc := nat.
+
+Variant envE (V : Type) :Type -> Type :=
+|GetE:   loc -> envE V V
+|PutE:   loc -> V -> envE V ()
+|AllocE: V -> envE V loc 
+|FreeE:  loc -> envE V ().
+
+
+Arguments GetE {_}.
+Arguments PutE {_}.
+Arguments AllocE {_}.
+Arguments FreeE {_}.
+
+Definition expr (V: Type) := itree (envE V). 
+
+Definition get {V} (l: nat): expr V V := Vis (GetE l) Answer.
+Definition put {V} (l: nat) (v: V): expr V () := Vis (PutE l v) Answer .
+Definition alloc {V} (v: V): expr V loc := Vis (AllocE v) Answer.
+Definition free {V} (l: loc): expr V () := Vis (FreeE l) Answer.
+
+
+(* Apply the continuation k to the Ret nodes of the itree t *)
+Instance itree_bind {E}: MBind (itree E) := λ R S k, 
+    cofix go u := match u with
+    | Answer r => k r
+    | Think t => Think (go t)
+    | Fork e k => Fork e (go k)
+    | Vis e k => Vis e (λ x, go (k x))
+    end.
+
+
+Instance itree_mret {E}: MRet (itree E) :=
  λ _ x, Answer x.
 
-Instance mbind_delayST ST : MBind (delayST ST) := 
- λ _ _ f ma, delayST_bind f ma.
-
-Instance fmap_delayST ST: FMap (delayST ST) :=
+Instance itree_fmap {E}: FMap (itree E) :=
    λ A B f ma, ma ≫= mret ∘ f.
 
+(* Definition delay_st_pipe {ST A B C} 
+    (f: A -> delay_st ST B)
+    (g: B -> delay_st ST C): A -> delay_st ST C := 
+  λ x,  f x ≫= g.
+
+Definition case_ {A B C}  (f: A -> C) (g: B -> C)
+  : (A + B -> C) :=
+    λ ab,
+        match ab with
+        | inl a => f a
+        | inr b => g b
+        end .
+  
+CoFixpoint iter {ST A B} (f: A -> delay_st ST (A + B)) : A -> delay_st ST B :=
+    delay_st_pipe f (case_ (Think ∘ iter f) Answer). *)
+
+
 (* do I want to use the state monad here or expose the pairs? *)
-Definition step_delayST {ST A} (e: delayST ST A): state ST (delayST ST A). 
-refine(
-    match e with
-    | Answer x  => mret $ Answer x 
-    | Get k     => k <$> getS 
-    | Put s' k  => k <$> putS s'
-    | Think e'  => mret e'
-    end
+
+Definition wp {Σ} {R V} (SI: gmap nat V -> iProp Σ) (e: expr V R) (Φ: R -> iProp Σ): iProp Σ.
+Admitted.
+
+Definition foo {V R} (c: envE V R) (σ σ': gmap loc V): R -> Prop.
+refine (match c with
+        |GetE l  => λ v, σ !! l = Some v /\ σ' = σ 
+        |PutE l v' => λ _, is_Some (σ !! l) /\ σ' = <[l := v']> σ
+        |AllocE v' => λ _, True
+        |FreeE l => λ _, True 
+        end
 ).
 Defined.
 
+Definition wp_pre {Σ} {V} (SI: gmap loc V -> iProp Σ)
+     (go: discrete_funO (λ R, expr V R -d> (R -d> iPropO Σ) -d> iPropO Σ)):
+     discrete_funO (λ R, expr V R -d> (R -d> iPropO Σ) -d> iPropO Σ).
+refine(λ R e Φ,
+        match e with
+        |Answer x => Φ x 
+        |Think e' => ▷ go R e' Φ
+        |Fork e' k => ▷ (go R k Φ ∗ go unit e' (λ _, True))
+        |Vis c k => ∀σ, SI σ ==∗ ∃σ' v, ⌜foo c σ σ' v⌝ ∗ SI σ' ∗ ▷ go _ (k v) Φ
+        end
+)%I.
+Defined.
+
+Instance wp_pre_contractive {Σ A SI}: Contractive (@wp_pre Σ A SI).
+Proof.
+  rewrite /wp_delay_pre => n wp wp' Hwp e1 Φ.
+  repeat (f_contractive || f_equiv); apply Hwp.
+Qed.
+ 
+Definition wp_delay {Σ} {A}: delay A -> (A -> iProp Σ)-> iProp Σ := fixpoint wp_delay_pre.
+
+Definition wp {Σ} {ST A} (SI: ST -> iProp Σ) (e: state_delay ST A) (Φ: A -> iProp Σ): iProp Σ.
+refine(∀ σ, 
+    SI σ ==∗
+     wp_delay (runState e σ) (λ (res: option (ST * A)), 
+       match res with   
+       | Some (σ', x) => SI σ' ∗ Φ x 
+       | None => True
+       end)
+)%I.
+Defined.
+
+Definition step_delay_st {ST A} (e: delay_st ST A): state ST (delay_st ST A) :=
+    match e with
+    | Answer x  => mret $ Answer x 
+    | Get n k     => k <$> getS 
+    | Put n s' k  => k <$> putS s'
+    | Think e'  => mret e'
+    end.
+
+Definition heap := gmap nat nat.
+
+Definition step_delay_st_heap {A} (e: delay_st heap A)
+    : state heap (delay_st heap A).
+refine (
+    match e with
+    | Answer x   => mret $ Answer x
+    | Get n k    => _
+    | Put n s' k => _
+    | Think e'   => _
+    end
+).
+- refine(_).
+Admitted.
+
 (* First a single threaded evaluator *)
-Fixpoint eval_delayST {ST A} (n: nat) (e: delayST ST A) (s: ST) {struct n} : option A :=
+Fixpoint eval_delay_st {ST A} (n: nat) (e: delay_st ST A) (s: ST) {struct n} : option A :=
     match n with
     | O => None
-    | S n' => match (runState (step_delayST e) s) with 
-              | Some (e', s') => eval_delayST n' e' s'
+    | S n' => match (runState (step_delay_st e) s) with 
+              | Some (e', s') => eval_delay_st n' e' s'
               | None => None
               end
     end.
@@ -73,41 +168,41 @@ Fixpoint split_and_circulate {A} (xs: list A) (f: A -> A) {struct xs}: (list A) 
     | cons x xs' => xs' ++ [f x]
     end.
 
-Definition step_delayST_threads {ST A} 
-    (threads: list (delayST ST A)) (s: ST)
-    :(ST * (list (delayST ST A))) :=
+Definition step_delay_st_threads {ST A} 
+    (threads: list (delay_st ST A)) (s: ST)
+    :(ST * (list (delay_st ST A))) :=
         match threads with 
         | nil => (s, nil)
-        | cons e es' => match (runState (step_delayST e) s) with
+        | cons e es' => match (runState (step_delay_st e) s) with
                         | None => (s, nil)
                         | Some (e', s') => (s', es' ++ [e'])
                         end
         end.
 
-Definition check_delayST {ST A} (e: delayST ST A): A + delayST ST A :=
+Definition check_delay_st {ST A} (e: delay_st ST A): A + delay_st ST A :=
     match e with
     | Answer x  => inl x
-    | Get k     => inr $ e
-    | Put s' k  => inr $ e
+    | Get n k     => inr $ e
+    | Put n s' k  => inr $ e
     | Think e'  => inr $ e
     end.
 
 (* Todo check the order of effects with list and state here
    and remove all these nested pattern matches
 *)
-Fixpoint eval_threaded_delayST {ST A} 
+Fixpoint eval_threaded_delay_st {ST A} 
     (n: nat) 
-    (threads: list (delayST ST A))
+    (threads: list (delay_st ST A))
     (s: ST) {struct n}: option A :=
 
     match n with
     | O => None
-    | S n' => let (s', threads') := (step_delayST_threads threads s)
+    | S n' => let (s', threads') := (step_delay_st_threads threads s)
               in match threads' with
                  | nil => None
-                 | cons e' _ => match check_delayST e' with
+                 | cons e' _ => match check_delay_st e' with
                                 | inl x => Some x
-                                | inr e'' => eval_threaded_delayST n' threads' s'
+                                | inr e'' => eval_threaded_delay_st n' threads' s'
                                 end
                  end
     end.
